refactor: `IsMonotone` to use `Ord`

Batteries/Data/RBMap/WF.lean
@@ -525,9 +525,9 @@ protected theorem Balanced.map {t : RBNode α} : t.Balanced c n → (t.map f).Ba
   | .black hl hr => .black hl.map hr.map
 
 /-- The property of a map function `f` which ensures the `map` operation is valid. -/
-class IsMonotone (cmpα cmpβ) (f : α → β) : Prop where
+class IsMonotone [Ord α] [Ord β] (f : α → β) : Prop where
   /-- If `x < y` then `f x < f y`. -/
-  lt_mono : cmpLT cmpα x y → cmpLT cmpβ (f x) (f y)
+  lt_mono : cmpLT compare x y → cmpLT compare (f x) (f y)
 
 /-- Sufficient condition for `map` to preserve an `All` quantifier. -/
 protected theorem All.map {f : α → β} (H : ∀ {x}, p x → q (f x)) :
@@ -536,8 +536,8 @@ protected theorem All.map {f : α → β} (H : ∀ {x}, p x → q (f x)) :
   | node .., ⟨hx, ha, hb⟩ => ⟨H hx, ha.map H, hb.map H⟩
 
 /-- The `map` function preserves the order invariants if `f` is monotone. -/
-protected theorem Ordered.map (f : α → β) [IsMonotone cmpα cmpβ f] :
-    ∀ {t : RBNode α}, t.Ordered cmpα → (t.map f).Ordered cmpβ
+protected theorem Ordered.map [Ord α] [Ord β] (f : α → β) [IsMonotone f] :
+    ∀ {t : RBNode α}, t.Ordered compare → (t.map f).Ordered compare
   | nil, _ => ⟨⟩
   | node _ a x b, ⟨ax, xb, ha, hb⟩ => by
     refine ⟨ax.map ?_, xb.map ?_, ha.map f, hb.map f⟩ <;> exact IsMonotone.lt_mono
@@ -553,7 +553,7 @@ This requires `IsMonotone` on the function in order to preserve the order invari
 If the function is not monotone, use `RBSet.map` instead.
 -/
 @[inline] def mapMonotone {α : Type u} {β : Type v} [Ord α] [Ord β]
-  (f : α → β) [IsMonotone compare compare f] (t : RBSet α) : RBSet β :=
+  (f : α → β) [IsMonotone f] (t : RBSet α) : RBSet β :=
   ⟨t.1.map f, have ⟨h₁, _, _, h₂⟩ := t.2.out; .mk (h₁.map _) h₂.map⟩
 
 end RBSet
@@ -571,8 +571,9 @@ We extract this as a function so that `IsMonotone (mapSnd f)` can be an instance
 
 open Ordering (byKey)
 
+open scoped Ordering in
 instance instIsMonotoneByKeyMapSnd [Ord α] (f : α → β → γ) :
-    IsMonotone (byKey Prod.fst) (byKey Prod.fst) (mapSnd f) where
+    @IsMonotone _ _ ⟨byKey Prod.fst⟩ ⟨byKey Prod.fst⟩ (mapSnd f) where
   lt_mono | ⟨h⟩ => ⟨@fun _ => @h {
     symm := fun (a₁, b₁) (a₂, b₂) =>
       OrientedCmp.symm (cmp := byKey Prod.fst) (a₁, f a₁ b₁) (a₂, f a₂ b₂)
